src/lib/communication/DY.Lib.Communication.RequestResponse.fst
@@ -74,27 +74,23 @@ type communication_reqres_event =
 %splice [ps_communication_reqres_event_is_well_formed] (gen_is_well_formed_lemma (`communication_reqres_event))
 #pop-options
 
-class comm_layer_event_reqres_tag = {
+class comm_layer_reqres_tag = {
   tag: string;
 }
 
-instance default_comm_layer_event_reqres_tag: comm_layer_event_reqres_tag = {
-  tag = "DY.Lib.Communication.Event.RequestResponse"
-}
-
-instance event_communication_reqres_event {|t:comm_layer_event_reqres_tag|}: event communication_reqres_event = {
+instance event_communication_reqres_event {|t:comm_layer_reqres_tag|}: event communication_reqres_event = {
   tag = t.tag;
   format = mk_parseable_serializeable ps_communication_reqres_event;
 }
 
-instance comm_layer_event_tag_core_reqres: comm_layer_event_core_tag = {
+instance comm_layer_tag_core_reqres: comm_layer_core_tag = {
   tag = "DY.Lib.Communication.Event.RequestResponse.Core"
 }
 
 (*** Layer Setup ***)
 
-val comm_layer_aead_tag: string
-let comm_layer_aead_tag = "DY.Lib.Communication.Aead.Key"
+val comm_layer_aead_tag: {|comm_layer_reqres_tag|} -> string
+let comm_layer_aead_tag #tag = tag.tag ^ ".Aead.Key"
 
 [@@with_bytes bytes]
 type comm_meta_data = {
@@ -112,12 +108,12 @@ type comm_meta_data = {
 
 [@@ "opaque_to_smt"]
 val send_request:
-  {|comm_layer_event_reqres_tag|} ->
+  {|comm_layer_reqres_tag|} ->
   #a:Type -> {| parseable_serializeable bytes a |} ->
   communication_keys_sess_ids ->
   principal -> principal -> a ->
   traceful (option (timestamp & comm_meta_data))
-let send_request #event_tag #a comm_keys_ids client server request =
+let send_request #tag #a comm_keys_ids client server request =
   let* key = mk_rand (AeadKey comm_layer_aead_tag empty) (comm_label client server) 32 in
   let payload_bytes = serialize #bytes a request in
   let* sid = new_session_id client in
@@ -130,12 +126,12 @@ let send_request #event_tag #a comm_keys_ids client server request =
 
 [@@ "opaque_to_smt"]
 val receive_request:
-  {|comm_layer_event_reqres_tag|} ->
+  {|comm_layer_reqres_tag|} ->
   #a:Type -> {| parseable_serializeable bytes a |} ->
   communication_keys_sess_ids ->
   principal -> timestamp ->
   traceful (option (a & comm_meta_data))
-let receive_request #event_tag #a comm_keys_ids server msg_id =
+let receive_request #tag #a comm_keys_ids server msg_id =
   let*? req_msg_t:com_message_t = receive_confidential comm_keys_ids server msg_id in
   guard_tr (RequestMessage? req_msg_t);*?
   let RequestMessage req_msg = req_msg_t in
@@ -174,10 +170,10 @@ let compute_response_message #a server key nonce response =
 
 [@@ "opaque_to_smt"]
 val send_response:
-  {|comm_layer_event_reqres_tag|} ->
+  {|comm_layer_reqres_tag|} ->
   #a:Type -> {| parseable_serializeable bytes a |} ->
   principal -> comm_meta_data -> a -> traceful (option timestamp)
-let send_response #event_tag #a server req_meta_data response =
+let send_response #tag #a server req_meta_data response =
   let*? state = get_state server req_meta_data.sid in
   guard_tr (ServerReceiveRequest? state);*?
   let ServerReceiveRequest srr = state in
@@ -191,10 +187,10 @@ let send_response #event_tag #a server req_meta_data response =
 
 [@@ "opaque_to_smt"]
 val decode_response_message:
-  {|comm_layer_event_reqres_tag|} ->
+  {|comm_layer_reqres_tag|} ->
   #a:Type -> {| parseable_serializeable bytes a |} ->
   principal -> bytes -> bytes -> option a
-let decode_response_message #event_tag #a server key msg_bytes =
+let decode_response_message #tag #a server key msg_bytes =
   let? resp_env_t:com_message_t = parse com_message_t msg_bytes in
   guard (ResponseMessage? resp_env_t);?
   let ResponseMessage resp_env = resp_env_t in
@@ -206,11 +202,11 @@ let decode_response_message #event_tag #a server key msg_bytes =
 
 [@@ "opaque_to_smt"]
 val receive_response:
-  {|comm_layer_event_reqres_tag|} ->
+  {|comm_layer_reqres_tag|} ->
   #a:Type -> {| parseable_serializeable bytes a |} ->
   principal -> comm_meta_data -> timestamp ->
   traceful (option (a & comm_meta_data))
-let receive_response #event_tag #a client req_meta_data msg_id =
+let receive_response #tag #a client req_meta_data msg_id =
   let*? state = get_state client req_meta_data.sid in
   guard_tr (ClientSendRequest? state);*?
   let ClientSendRequest csr = state in
